ZtoConflNom.v
@@ -1,0 +1,300 @@
+(** * The Z property implies Confluence in the Nominal setting *)
+
+(* begin hide *)
+Definition Rel (A:Type) := A -> A -> Prop.
+
+Inductive trans {A} (red: Rel A) : Rel A :=
+| singl: forall a b,  red a b -> trans red a b
+| transit: forall b a c,  red a b -> trans red b c -> trans red a c.
+
+Arguments transit {A} {red} _ _ _ _ _ .
+
+Lemma trans_composition {A} (R: Rel A):
+  forall t u v, trans R t u -> trans R u v -> trans R t v.
+Proof.
+  intros t u v H1 H2. induction H1.
+  - apply transit with b; assumption.
+  - apply transit with b.
+    + assumption.
+    + apply IHtrans; assumption.
+Qed.
+
+Lemma transit_composition' {A:Type} (R: Rel A):
+  forall t u v, trans R t u -> R u v -> trans R t v.
+Proof.
+  intros t u v H1 H2. induction H1.
+  - apply transit with b.
+    + assumption.
+    + apply singl. assumption.
+  - apply IHtrans in H2.
+    apply transit with b; assumption.
+Qed.
+
+Lemma trans_composition' {A} (R: Rel A):
+  forall t v, trans R t v -> (R t v \/ exists u, trans R t u /\ R u v).
+Proof.
+ intros t v H.
+ induction H.
+ - left; assumption.
+ - right.
+   destruct IHtrans.
+   + exists b.
+     split.
+     * apply singl.
+       assumption.
+     * assumption.
+   + destruct H1.
+     exists x.
+     split.
+     * apply transit with b.
+       ** assumption.
+       ** apply H1.
+     * apply H1.
+Qed.
+(* end hide *)
+
+Inductive refltrans {A:Type} (R: Rel A) : A -> A -> Prop :=
+| refl: forall a, (refltrans R) a a
+| rtrans: forall a b c, R a b -> refltrans R b c -> refltrans R a c.
+
+Lemma refltrans_composition {A} (R: Rel A): forall t u v, refltrans R t u -> refltrans R u v -> refltrans R t v.
+Proof.  
+  intros t u v.  
+  intros H1 H2.
+  induction H1.
+  - assumption.
+  - apply rtrans with b.
+    + assumption.
+    + apply IHrefltrans; assumption.  
+Qed. 
+
+(* begin hide *)
+Lemma refltrans_composition2 {A} (R: Rel A): forall t u v, refltrans R t u -> R u v -> refltrans R t v.
+Proof.
+  intros t u v H1 H2. induction H1.
+  - apply rtrans with v.
+    + assumption.
+    + apply refl.
+  - apply IHrefltrans in H2.
+    apply rtrans with b; assumption.
+Qed.
+
+Lemma trans_to_refltrans {A:Type} (R: Rel A): forall a b, trans R a b -> refltrans R a b.
+Proof.
+  intros a b Htrans.
+  induction Htrans.
+  - apply rtrans with b.
+    + assumption.
+    + apply refl.
+  - apply rtrans with b; assumption.
+Qed.    
+(* end hide *)
+
+Definition Confl {A:Type} (R: Rel A) := forall a b c, (refltrans R) a b -> (refltrans R) a c -> (exists d, (refltrans R) b d /\ (refltrans R) c d).
+
+Definition Z_prop {A:Type} (R: Rel A) := exists f:A -> A, forall a b, R a b -> ((refltrans R) b (f a) /\ (refltrans R) (f a) (f b)).
+
+Definition f_is_Z {A:Type} (R: Rel A) (f: A -> A) := forall a b, R a b -> ((refltrans R)  b (f a) /\ (refltrans R) (f a) (f b)). 
+
+Theorem Z_prop_implies_Confl {A:Type}: forall R: Rel A, Z_prop R -> Confl R.
+Proof.
+  intros R HZ_prop. unfold Z_prop, Confl in *. intros a b c Hrefl1 Hrefl2.
+  destruct HZ_prop as [g HZ_prop].
+  generalize dependent c. 
+  induction Hrefl1. 
+  - intros c Hrefl2. 
+    exists c; split. 
+    + assumption. 
+    + apply refl. 
+  - intros c0 Hrefl2. 
+    assert (Hbga: refltrans R b (g a)).
+    { apply HZ_prop; assumption.  } 
+    assert (Haga: refltrans R a (g a)).
+    { apply rtrans with b; assumption.  } 
+    clear H. generalize dependent b. induction Hrefl2. 
+    + intros b Hrefl1 IHHrefl1 Hbga. 
+      assert (IHHrefl1_ga := IHHrefl1 (g a)); apply IHHrefl1_ga in Hbga. 
+      destruct Hbga. 
+      exists x; split. 
+      * apply H. 
+      * apply refltrans_composition with (g a); [assumption | apply H]. 
+    + intros b0 Hrefl1 IHHrefl1 Hb0ga. apply IHHrefl2 with b0.
+      * apply refltrans_composition with (g a); apply HZ_prop; assumption. 
+      * assumption.
+      * assumption.
+      * apply refltrans_composition with (g a); [ assumption | apply HZ_prop; assumption]. 
+Qed.
+  
+Definition SemiConfl {A:Type} (R: Rel A) := forall a b c, R a b -> (refltrans R) a c -> (exists d, (refltrans R) b d /\ (refltrans R) c d).
+
+Theorem Z_prop_implies_SemiConfl {A:Type}: forall R: Rel A, Z_prop R -> SemiConfl R.
+(* begin hide *)
+Proof.
+  intros R HZ_prop.
+  unfold Z_prop in HZ_prop.
+  unfold SemiConfl.
+  destruct HZ_prop.
+  intros a b c Hrefl Hrefl'.
+  assert (Haxa: refltrans R a (x a)).
+  { apply rtrans with b.  - assumption.  - apply H.  assumption.  }
+  apply H in Hrefl.
+  destruct Hrefl.
+  clear H1.
+  generalize dependent b.
+  induction Hrefl'.
+  - intros.
+    exists (x a).
+    split; assumption.
+  - intros.
+    destruct IHHrefl' with b0.
+    + apply refltrans_composition with (x a); apply H; assumption.
+    + apply refltrans_composition with (x b).
+      * apply refltrans_composition with (x a).
+        ** assumption.
+        ** apply H.
+           assumption.
+      * apply refl.
+    + exists x0.
+      assumption.
+Qed.
+(* end hide *)
+
+Theorem Semi_equiv_Confl {A: Type}: forall R: Rel A, Confl R <-> SemiConfl R.
+(* begin hide *)
+Proof.
+  unfold Confl.
+  unfold SemiConfl.
+  intro R.
+  split.
+  - intros.
+    apply H with a.
+    + apply rtrans with b.
+      * assumption.
+      * apply refl.
+    + assumption.
+  - intros.
+    generalize dependent c.
+    induction H0.
+    + intros.
+      exists c.
+      split.
+      * assumption.
+      * apply refl.
+    + intros.
+      specialize (H a).
+      specialize (H b).
+      specialize (H c0).
+      apply H in H0.
+      * destruct H0.
+        destruct H0.
+        apply IHrefltrans in H0.
+        destruct H0.
+        destruct H0.
+        exists x0.
+        split.
+        ** assumption.
+        ** apply refltrans_composition with x; assumption.
+      * assumption.
+Qed.
+(* end hide *)
+
+Corollary Zprop_implies_Confl_via_SemiConfl {A:Type}: forall R: Rel A, Z_prop R -> Confl R.
+Proof. intros R HZ_prop. apply Semi_equiv_Confl. generalize dependent HZ_prop.
+       apply Z_prop_implies_SemiConfl. Qed.
+
+(** * An extension of the Z property: Compositional Z *)
+
+Definition f_is_weak_Z {A} (R R': Rel A) (f: A -> A) := forall a b, R a b -> ((refltrans R') b (f a) /\ (refltrans R') (f a) (f b)).
+
+Definition comp {A} (f1 f2: A -> A) := fun x:A => f1 (f2 x).
+Notation "f1 # f2" := (comp f1 f2) (at level 40).
+
+Inductive union {A} (red1 red2: Rel A) : Rel A :=
+| union_left: forall a b, red1 a b -> union red1 red2 a b
+| union_right: forall a b, red2 a b -> union red1 red2 a b.
+Notation "R1 !_! R2" := (union R1 R2) (at level 40).
+
+(* begin hide *)
+Lemma union_or {A}: forall (r1 r2: Rel A) (a b: A), (r1 !_! r2) a b <-> (r1 a b) \/ (r2 a b).
+Proof.
+  intros r1 r2 a b; split.
+  - intro Hunion.
+    inversion Hunion; subst.
+    + left; assumption.
+    + right; assumption.
+  - intro Hunion.
+    inversion Hunion.
+    + apply union_left; assumption.
+    + apply union_right; assumption.
+Qed.
+(* end hide *)
+
+(** We are now ready to present the definition of the compositional Z:
+
+    %\begin{theorem}\cite{Nakazawa-Fujita2016}\label{thm:zcomp} Let
+     $(A,\to_R)$ be an ARS such that $\to_R = \to_1 \cup \to_2$. If
+     there exists mappings $f_1,f_2: A \to A$ such that
+     \begin{enumerate} \item $f_1$ is Z for $\to_1$ \item $a \to_1 b$
+     implies $f_2(a) \tto f_2(b)$ \item $a \tto f_2(a)$ holds for any
+     $a\in Im(f_1)$ \item $f_2 \circ f_1$ is weakly Z for $\to_2$ by
+     $\to_R$ \end{enumerate} then $f_2 \circ f_1$ is Z for
+     $(A,\to_R)$, and hence $(A,\to_R)$ is confluent.  \end{theorem}%
+
+    We define the predicate [Z_comp] that corresponds to the premises
+    of Theorem %\ref{thm:zcomp}%, i.e. to the conjunction of items
+    (i), (ii), (iii) and (iv) in addition to the fact that $\to_R =
+    \to_1 \cup \to_2$, where $\to_1$ (resp. $\to_2$) is written as
+    [R1] (resp. [R2]): *)
+
+Definition Z_comp {A:Type} (R :Rel A) := exists (R1 R2: Rel A) (f1 f2: A -> A), (forall x y, R x y <-> (R1 !_! R2) x y) /\ f_is_Z R1 f1 /\ (forall a b, R1 a b -> (refltrans R) (f2 a) (f2 b)) /\ (forall a b, b = f1 a -> (refltrans R) b (f2 b)) /\ (f_is_weak_Z R2 R (f2 # f1)).
+
+(* begin hide *)
+Lemma refltrans_union {A:Type}: forall (R R' :Rel A) (a b: A), refltrans R a b -> refltrans (R !_! R') a b.
+Proof.
+  intros R R' a b Hrefl.
+  induction Hrefl.
+  - apply refl.
+  - apply rtrans with b.
+    + apply union_left; assumption.
+    + assumption.
+Qed.
+(* end hide *)
+
+Lemma refltrans_union_equiv {A}: forall (R R1 R2 : Rel A) (x y : A), R x y <-> (R1 !_! R2) x y -> forall x y : A, refltrans (R1 !_! R2) x y -> refltrans R x y.
+Proof.  
+Admitted.
+  
+Theorem Z_comp_implies_Z_prop {A:Type}: forall (R :Rel A), Z_comp R -> Z_prop R.
+Proof.
+  intros R H.
+  unfold Z_prop. unfold Z_comp in H. destruct H as
+  [ R1 [ R2 [f1 [f2 [Hunion [H1 [H2 [H3 H4]]]]]]]]. 
+  exists (f2 # f1). 
+  intros a b HR.
+  apply Hunion in HR. inversion HR; subst. clear HR.
+  - split. 
+    + apply refltrans_composition with (f1 a). 
+      * apply H1 in H.
+        destruct H as [Hb Hf].
+        apply (refltrans_union R1 R2) in Hb.
+        apply refltrans_union_equiv with R1 R2 b (f1 a).
+        ** apply Hunion.
+        ** apply Hb.
+      * apply H3 with a; reflexivity. 
+    + apply H1 in H.  destruct H as [Hb Hf].
+      clear Hb.  unfold comp. 
+      induction Hf. 
+      * apply refl. 
+      * apply refltrans_composition with (f2 b0). 
+        ** apply H2; assumption. 
+        ** apply IHHf. 
+  - apply H4; assumption. 
+Qed.
+
+Corollary Z_comp_is_Confl {A}: forall (R: Rel A), Z_comp R -> Confl R.
+Proof.
+  intros R H.
+  apply Z_comp_implies_Z_prop in H.
+  apply Z_prop_implies_Confl; assumption.
+Qed.
+
